q

DL/DL_Basics.ec
@@ -1,3 +1,4 @@
+pragma Goals:printall.
 require import AllCore Distr DInterval.
 require import AllCore DBool Bool List Int IntDiv.
 
@@ -10,6 +11,11 @@ type dl_com = int.
 type dl_resp = int.
 
 op IsPrime : int -> bool.
+
+op VerifyZK : dl_prob -> dl_com -> dl_resp -> bool.
+op VerifyWit : dl_prob -> dl_wit -> bool.
+op ExtractWit : dl_prob -> dl_com -> dl_resp -> dl_resp -> dl_wit option.
+
 
 
 axiom dl_prop1 (p a x : int) : IsPrime p => a ^ x %% p = a ^ (x %% (p - 1)) %% p. 
@@ -64,11 +70,19 @@ module DL_HV : Verifier = {
   }
 
   proc verify(c : dl_com, r : dl_resp) : bool = {
+   
     return pa.`2 ^ r %% pa.`1 = ca * (if b then pa.`3 else 1) %% pa.`1;
  } 
 
  proc summitup(c : dl_com, r : dl_resp) : sbits = {
    return witness;
+ }
+
+ proc getState() : sbits = {
+   return witness;
+ }
+
+ proc setState(s : sbits) : unit = {
  }
 }.
 
@@ -91,6 +105,146 @@ have ->: A ^ (r1 + w{hr})
  = A ^ r1 * A^ w{hr}. apply exprD_nneg. smt. smt.   
 smt (modz_mod modzMml modzMmr modzMm).
 qed.   
+
+
+require RewWithInit.
+clone import RewWithInit.RWI as MRWI with type sbits <- sbits,
+                                          type iat   <- dl_prob,
+                                          type irt   <- dl_prob * dl_com,
+                                          type rrt   <- (bool * bool).
+
+
+module MyInit(P : Prover) : RW.Initializer = {
+  proc init(i : dl_prob)   = {
+    var c : dl_com;
+    c <- P.commit(i,witness);
+    return (i,c);
+  }
+}.                                  
+
+
+module MyRewRun(P : Prover) : RW.RewRun = {
+
+  proc run(pa : dl_prob, ca : dl_com) = {
+    var b : bool;
+    var r : dl_resp;
+    b <$ {0,1};
+
+    r <- P.response(b);
+    
+    return (b, pa.`2 ^ r %% pa.`1 = ca * (if b then pa.`3 else 1) %% pa.`1);
+  }
+
+  proc setState(s : sbits) = {
+    P.setState(s);
+  }
+  
+  proc getState() : sbits = {
+    return witness;
+  }
+}.
+
+
+section.
+declare module P : Prover.
+
+lemma step1 &m : forall (i : dl_prob),
+        Pr[QQ(MyRewRun(P), MyInit(P)).main_run(i) @ &m : snd (snd res)] ^ 2 <=
+        Pr[QQ(MyRewRun(P), MyInit(P)).main(i) @ &m : snd (snd res.`1) /\ snd (snd res.`2)].
+proof. move => i.
+apply (rew_with_init (MyRewRun(P)) (MyInit(P)) _ _ _ _ _ &m (fun x => snd (snd x ))).
+sim. sim. admit. admit. admit.
+qed.
+
+
+lemma step2 &m : forall (i : dl_prob),
+    Pr[QQ(MyRewRun(P), MyInit(P)).main_run(i) @ &m : snd (snd res)] ^ 2 <=
+    Pr[QQ(MyRewRun(P), MyInit(P)).main(i)
+      @ &m : (snd (snd res.`1) /\ snd (snd res.`2))
+         /\ res.`1.`2.`1 = res.`2.`2.`1 ]
+   + Pr[QQ(MyRewRun(P), MyInit(P)).main(i)
+      @ &m : (snd (snd res.`1) /\ snd (snd res.`2))
+         /\ res.`1.`2.`1 <> res.`2.`2.`1].
+proof. move => i.
+have <-: Pr[QQ(MyRewRun(P), MyInit(P)).main(i) @ &m :
+             (snd (snd res.`1) /\ snd (snd res.`2)) ] =
+   Pr[QQ(MyRewRun(P), MyInit(P)).main(i)
+      @ &m : (snd (snd res.`1) /\ snd (snd res.`2))
+         /\ res.`1.`2.`1 = res.`2.`2.`1 ]
+   + Pr[QQ(MyRewRun(P), MyInit(P)).main(i)
+      @ &m : (snd (snd res.`1) /\ snd (snd res.`2))
+         /\ res.`1.`2.`1 <> res.`2.`2.`1].
+rewrite Pr[mu_split res.`1.`2.`1 = res.`2.`2.`1]. 
+auto.
+apply step1.
+qed.
+
+lemma step3 &m : forall (i : dl_prob),
+ Pr[QQ(MyRewRun(P), MyInit(P)).main(i)
+     @ &m : (snd (snd res.`1) /\ snd (snd res.`2))
+        /\ res.`1.`2.`1 <> res.`2.`2.`1] >= 
+ Pr[QQ(MyRewRun(P), MyInit(P)).main_run(i) @ &m : snd (snd res)] ^ 2
+  -     Pr[QQ(MyRewRun(P), MyInit(P)).main(i)
+      @ &m : (snd (snd res.`1) /\ snd (snd res.`2))
+         /\ res.`1.`2.`1 = res.`2.`2.`1 ].
+smt (step2).
+qed.  
+
+
+lemma qwe &m i :
+ Pr[QQ(MyRewRun(P), MyInit(P)).main(i) @ &m : res.`1.`2.`1 = res.`2.`2.`1 ]
+ = 1%r/2%r.
+proof. byphoare. proc.
+inline*. simplify. wp. simplify.
+swap 6 -5. swap 12 -11.
+seq 2 : (b0 = b) (1%r/2%r) 1%r 1%r 0%r.
+admitted.
+
+
+lemma step4 &m : forall (i : dl_prob),
+ Pr[QQ(MyRewRun(P), MyInit(P)).main(i)
+     @ &m : (snd (snd res.`1) /\ snd (snd res.`2))
+        /\ res.`1.`2.`1 <> res.`2.`2.`1] >= 
+ Pr[QQ(MyRewRun(P), MyInit(P)).main_run(i) @ &m : snd (snd res)] ^ 2
+    - 1%r/2%r.
+move => i.
+have f : Pr[QQ(MyRewRun(P), MyInit(P)).main(i)
+      @ &m : (snd (snd res.`1) /\ snd (snd res.`2))
+         /\ res.`1.`2.`1 = res.`2.`2.`1 ] <= 1%r/2%r.
+rewrite - (qwe &m i).
+rewrite Pr[mu_sub]. progress. auto.
+smt (step3).
+qed.
+
+
+(*
+TODO:
+1/ embed verification into  (instead of just bools)
+
+ Pr[QQ(MyRewRun(P), MyInit(P)).main(i)
+     @ &m : (snd (snd res.`1) /\ snd (snd res.`2))
+        /\ res.`1.`2.`1 <> res.`2.`2.`1] 
+
+2/ show that if verification  succeeds and chals are different
+then  the above prob is equal to same probability but with
+witness extraction
+
+3/ assuming that single run succeeds with prob > sqrt(1/2) we
+have extraction prob > 0.
+
+4/ prove that there exists "p" equal to that prob and p > 0
+
+5/ apply "whp_cap_fin" to show the probability of extraction
+on i-th iteration.
+
+======
+
+
+
+*)
+
+
+
 
 
 (*
